refactor(library/nat): rename nat.le to nat.less_than
Motivation: avoid overload when we use `open nat`.

Unfortunately, we currently do not allow users to mark inductive datatype
declarations as protected.

library/init/nat.lean
@@ -11,13 +11,14 @@ notation `ℕ` := nat
 
 namespace nat
 
-inductive le (a : ℕ) : ℕ → Prop
-| nat_refl : le a    -- use nat_refl to avoid overloading le.refl
-| step : Π {b}, le b → le (succ b)
+inductive less_than (a : ℕ) : ℕ → Prop
+| refl : less_than a
+| step : Π {b}, less_than b → less_than (succ b)
 
 instance : has_le ℕ :=
-⟨nat.le⟩
+⟨nat.less_than⟩
 
+@[reducible] protected def le (n m : ℕ) := n ≤ m
 @[reducible] protected def lt (n m : ℕ) := succ n ≤ m
 
 instance : has_lt ℕ :=
@@ -61,17 +62,17 @@ instance : inhabited ℕ :=
 /- properties of inequality -/
 
 @[refl] protected def le_refl : ∀ a : ℕ, a ≤ a :=
-le.nat_refl
+less_than.refl
 
 lemma le_succ (n : ℕ) : n ≤ succ n :=
-le.step (nat.le_refl n)
+less_than.step (nat.le_refl n)
 
 lemma succ_le_succ {n m : ℕ} : n ≤ m → succ n ≤ succ m :=
-λ h, le.rec (nat.le_refl (succ n)) (λ a b, le.step) h
+λ h, less_than.rec (nat.le_refl (succ n)) (λ a b, less_than.step) h
 
 lemma zero_le : ∀ (n : ℕ), 0 ≤ n
 | 0     := nat.le_refl 0
-| (n+1) := le.step (zero_le n)
+| (n+1) := less_than.step (zero_le n)
 
 lemma zero_lt_succ (n : ℕ) : 0 < succ n :=
 succ_le_succ (zero_le n)
@@ -82,7 +83,9 @@ lemma not_succ_le_zero : ∀ (n : ℕ), succ n ≤ 0 → false
 lemma not_lt_zero (a : ℕ) : ¬ a < 0 := not_succ_le_zero a
 
 lemma pred_le_pred {n m : ℕ} : n ≤ m → pred n ≤ pred m :=
-λ h, le.rec (nat.le_refl (pred n)) (λ n, nat.rec (λ a b, b) (λ a b c, le.step) n) h
+λ h, less_than.rec_on h
+  (nat.le_refl (pred n))
+  (λ n, nat.rec (λ a b, b) (λ a b c, less_than.step) n)
 
 lemma le_of_succ_le_succ {n m : ℕ} : succ n ≤ succ m → n ≤ m :=
 pred_le_pred
@@ -100,7 +103,7 @@ instance decidable_lt : ∀ a b : ℕ, decidable (a < b) :=
 λ a b, nat.decidable_le (succ a) b
 
 protected lemma eq_or_lt_of_le {a b : ℕ} (h : a ≤ b) : a = b ∨ a < b :=
-le.cases_on h (or.inl rfl) (λ n h, or.inr (succ_le_succ h))
+less_than.cases_on h (or.inl rfl) (λ n h, or.inr (succ_le_succ h))
 
 lemma lt_succ_of_le {a b : ℕ} : a ≤ b → a < succ b :=
 succ_le_succ
@@ -117,11 +120,11 @@ protected lemma lt_irrefl (n : ℕ) : ¬n < n :=
 not_succ_le_self n
 
 protected lemma le_trans {n m k : ℕ} (h1 : n ≤ m) : m ≤ k → n ≤ k :=
-le.rec h1 (λ p h2, le.step)
+less_than.rec h1 (λ p h2, less_than.step)
 
 lemma pred_le : ∀ (n : ℕ), pred n ≤ n
-| 0        := le.nat_refl 0
-| (succ a) := le.step (le.nat_refl a)
+| 0        := less_than.refl 0
+| (succ a) := less_than.step (less_than.refl a)
 
 lemma sub_le (a b : ℕ) : a - b ≤ a :=
 nat.rec_on b (nat.le_refl (a - 0)) (λ b₁, nat.le_trans (pred_le (a - b₁)))
