tests/lean/concrete_instance.lean
@@ -5,8 +5,8 @@ set_option pp.all true
 check a * b
 check a + b
 
-instance : semigroup nat := sorry
-instance : add_semigroup nat := sorry
+-- instance : semigroup nat := sorry
+-- instance : add_semigroup nat := sorry
 
 check a * b
 check a + b
