tests/lean/protected_test.lean
@@ -2,10 +2,10 @@ namespace nat
   check induction_on      -- ERROR
   check rec_on            -- ERROR
   check nat.induction_on
-  check le.rec_on         -- OK
-  check nat.le.rec_on
+  check less_than.rec_on         -- OK
+  check nat.less_than.rec_on
   namespace le
     check rec_on          -- ERROR
-    check le.rec_on
+    check less_than.rec_on
   end le
 end nat
